PQXDH/Aeneas/Full/UAKE/Security.lean
@@ -1,0 +1,49 @@
+/-
+Copyright (c) 2026 Galois Inc. All rights reserved.
+Released under Apache 2.0 license as described in the file LICENSE.
+Authors: Ben Hamlin
+-/
+import PQXDH.Aeneas.Full.UAKE.SecurityLemmas
+
+open OracleSpec OracleComp AKE AKE.UAKE
+open libsignal_protocol
+
+namespace PQXDH.Aeneas.Full
+
+noncomputable section
+
+variable {Rand SPK SSK S C Msg IdC IdK : Type}
+
+theorem uakeInitiator_secure_pq
+    [DecidableEq S] [DecidableEq C] [DecidableEq Msg] [DecidableEq IdC] [DecidableEq IdK]
+    [Inhabited S] [Inhabited SSK]
+    (P : Parameters Rand SPK SSK S C Msg IdC IdK) (msg : Msg) (hasOPK : Bool)
+    (hidKEM : Function.Injective P.idKEM)
+    (A : UAKE.Adversary (uakeInitiator P msg hasOPK)) (q : ℕ) (hq : A.OpensAtMost q)
+    (εsig εkem εaead εkdf : ℝ)
+    (hkemCorrect : (pqkem P).PerfectlyCorrect ProbCompRuntime.probComp)
+    (hsig : ∀ B : P.sig.unforgeableAdv,
+      (B.strongAdvantage ProbCompRuntime.probComp).toReal ≤ εsig)
+    (hkem : ∀ B : (pqkem P).IND_CCA_Adversary,
+      KEMScheme.IND_CCA_Advantage ProbCompRuntime.probComp B ≤ εkem)
+    (haead : ∀ B : AEAD.INT_CTXT_D_Adversary P.aead,
+      AEAD.INT_CTXT_D_Advantage P.aead B ≤ εaead) :
+    UAKE.advantage A ≤ εsig + εkem + εaead + εkdf := sorry
+
+theorem uakeInitiator_secure_dh
+    [DecidableEq S] [DecidableEq C] [DecidableEq Msg] [DecidableEq IdC] [DecidableEq IdK]
+    [Inhabited S] [Inhabited SSK]
+    (P : Parameters Rand SPK SSK S C Msg IdC IdK) (msg : Msg) (hasOPK : Bool)
+    (hidEC : Function.Injective P.idEC)
+    (A : UAKE.Adversary (uakeInitiator P msg hasOPK)) (q : ℕ) (hq : A.OpensAtMost q)
+    (εsig εdh εaead εkdf : ℝ)
+    (hkemCorrect : (pqkem P).PerfectlyCorrect ProbCompRuntime.probComp)
+    (hsig : ∀ B : P.sig.unforgeableAdv,
+      (B.strongAdvantage ProbCompRuntime.probComp).toReal ≤ εsig)
+    (haead : ∀ B : AEAD.INT_CTXT_D_Adversary P.aead,
+      AEAD.INT_CTXT_D_Advantage P.aead B ≤ εaead) :
+    UAKE.advantage A ≤ εsig + εdh + εaead + εkdf := sorry
+
+end
+
+end PQXDH.Aeneas.Full
