PQXDH/Aeneas/Full/UAKE/SecurityLemmas.lean
@@ -1,0 +1,27 @@
+/-
+Copyright (c) 2026 Galois Inc. All rights reserved.
+Released under Apache 2.0 license as described in the file LICENSE.
+Authors: Ben Hamlin
+-/
+import PQXDH.Aeneas.Full.UAKE.Defs
+
+open OracleSpec OracleComp AKE AKE.UAKE
+open libsignal_protocol
+
+namespace PQXDH.Aeneas.Full
+
+noncomputable section
+
+variable {Rand SPK SSK S C Msg IdC IdK : Type}
+
+def specParams (P : Parameters Rand SPK SSK S C Msg IdC IdK) (F : Type) (gen : ECPub) :
+    PQXDH.Parameters F ECPub Key PQPub PQPriv CT SPK SSK S C Msg Key IdC IdK := sorry
+
+structure ECGroupModel {F : Type} [Field F] [SampleableType F]
+    [AddCommGroup ECPub] [Module F ECPub]
+    (P : Parameters Rand SPK SSK S C Msg IdC IdK) (gen : ECPub)
+    (privEnc : F → ECPriv) : Prop where
+
+end
+
+end PQXDH.Aeneas.Full
