PQXDH/Aeneas/Simplified/UAKE.lean
@@ -1,0 +1,14 @@
+/-
+Copyright (c) 2026 Galois Inc. All rights reserved.
+Released under Apache 2.0 license as described in the file LICENSE.
+Authors: Ben Hamlin
+-/
+import PQXDH.Aeneas.Simplified.UAKE.Defs
+import PQXDH.Aeneas.Simplified.UAKE.CorrectnessLemmas
+import PQXDH.Aeneas.Simplified.UAKE.Correctness
+import PQXDH.Aeneas.Simplified.UAKE.SecurityLemmas
+import PQXDH.Aeneas.Simplified.UAKE.Security
+
+/-!
+# PQXDH as a UAKE, instantiated with the Aeneas-extracted implementation
+-/
