PQXDH/Aeneas/Simplified/UAKE/Defs.lean
@@ -1,0 +1,303 @@
+/-
+Copyright (c) 2026 Galois Inc. All rights reserved.
+Released under Apache 2.0 license as described in the file LICENSE.
+Authors: Ben Hamlin
+-/
+import PQXDH.Aeneas.Simplified.Extracted.Pqxdh
+import PQXDH.Spec.Basic
+import PQXDH.Spec.UAKE
+import ToVCVio.CryptoFoundations.AKE.UAKE.Defs
+import ToVCVio.CryptoFoundations.AKE.UAKE.Transport
+import ToVCVio.CryptoFoundations.HardnessAssumptions.DiffieHellman
+
+/-!
+# PQXDH as a UAKE, instantiated with the Aeneas-extracted implementation
+-/
+
+open OracleSpec OracleComp AKE AKE.UAKE
+
+namespace PQXDH.Aeneas.Simplified
+
+noncomputable section
+
+instance {α : Type} {n : Aeneas.Std.Usize} [DecidableEq α] :
+    DecidableEq (Aeneas.Std.Array α n) :=
+  inferInstanceAs (DecidableEq { l : List α // l.length = n.val })
+
+instance : SampleableType Aeneas.Std.U8 :=
+  SampleableType.ofEquiv (α := BitVec 8)
+    ⟨fun bv => ⟨bv⟩, fun x => x.bv, fun _ => rfl, fun _ => rfl⟩
+
+instance {α : Type} {n : Aeneas.Std.Usize} [SampleableType α] :
+    SampleableType (Aeneas.Std.Array α n) :=
+  inferInstanceAs (SampleableType (List.Vector α n.val))
+
+instance : Fintype Aeneas.Std.U8 :=
+  Fintype.ofEquiv (BitVec 8) ⟨fun bv => ⟨bv⟩, fun x => x.bv, fun _ => rfl, fun _ => rfl⟩
+
+instance {α : Type} {n : Aeneas.Std.Usize} [Fintype α] :
+    Fintype (Aeneas.Std.Array α n) :=
+  inferInstanceAs (Fintype (List.Vector α n.val))
+
+abbrev Bytes (n : Aeneas.Std.Usize) : Type := Aeneas.Std.Array Aeneas.Std.U8 n
+
+abbrev ECKey : Type := Bytes 32#usize
+
+abbrev PQPK : Type := Bytes 1568#usize
+
+abbrev PQSK : Type := Bytes 3168#usize
+
+abbrev CT : Type := Bytes 1569#usize
+
+abbrev SS : Type := Bytes 32#usize
+
+abbrev Key : Type := Bytes 32#usize
+
+abbrev Coins : Type := Bytes 32#usize
+
+def getOk {α : Type} [Inhabited α] : Aeneas.Std.Result α → α
+  | .ok x => x
+  | _ => default
+
+def deriveKeys (dh1 dh2 dh3 : ECKey) (dh4 : Option ECKey) (ss : SS) :
+    Aeneas.Std.Result (Key × Key × Key) := do
+  let okm ← match dh4 with
+    | none => do
+        let secretInput ← pqxdh.pqxdh_secret_input dh1 dh2 dh3 ss
+        let s ← Aeneas.Std.lift (Aeneas.Std.Array.to_slice secretInput)
+        let s1 ← Aeneas.Std.lift (Aeneas.Std.Array.to_slice pqxdh.PQXDH_LABEL)
+        pqxdh.hkdf_sha256_derive s s1
+    | some dh4 => do
+        let secretInput ← pqxdh.pqxdh_secret_input_with_opk dh1 dh2 dh3 dh4 ss
+        let s ← Aeneas.Std.lift (Aeneas.Std.Array.to_slice secretInput)
+        let s1 ← Aeneas.Std.lift (Aeneas.Std.Array.to_slice pqxdh.PQXDH_LABEL)
+        pqxdh.hkdf_sha256_derive s s1
+  pqxdh.derive_split okm
+
+def DeriveKeysTotal : Prop :=
+  ∀ (dh1 dh2 dh3 : ECKey) (dh4 : Option ECKey) (ss : SS),
+    ∃ ks, deriveKeys dh1 dh2 dh3 dh4 ss = .ok ks
+
+variable {SPK SSK S C Msg IdC IdK : Type}
+
+structure Parameters (SPK SSK S C Msg IdC IdK : Type) where
+  ecKeygen : ProbComp pqxdh.KeyPair
+  pqKeygen : ProbComp (PQPK × PQSK)
+  encapsCoins : ProbComp Coins
+  sig : SignatureAlg ProbComp (ECKey ⊕ PQPK) SPK SSK S
+  aead : AEAD.Scheme ProbComp Msg Key (ECKey × ECKey × PQPK) C
+  idEC : ECKey → IdC
+  idKEM : PQPK → IdK
+
+structure InitiatorParameters (SPK Msg : Type) where
+  ikA : pqxdh.KeyPair
+  ikB : ECKey
+  sigpkB : SPK
+  msg : Msg
+
+structure RecipientIdentity (SPK SSK S : Type) where
+  ikB : pqxdh.KeyPair
+  sigkB : SPK × SSK
+  spkB : pqxdh.KeyPair
+  spkSigB : S
+
+structure RecipientParameters (SPK SSK S : Type) where
+  ikB : pqxdh.KeyPair
+  sigkB : SPK × SSK
+  spkB : pqxdh.KeyPair
+  spkSigB : S
+  opkB : Option pqxdh.KeyPair
+  pqpkB : PQPK × PQSK
+
+def pqkem (P : Parameters SPK SSK S C Msg IdC IdK) :
+    KEMScheme ProbComp SS PQPK PQSK CT where
+  keygen := P.pqKeygen
+  encaps := fun pk => do
+    let coins ← P.encapsCoins
+    match pqxdh.mlkem_encapsulate pk coins with
+    | .ok (ss, ct) => return (ct, ss)
+    | _ => return default
+  decaps := fun sk ct =>
+    match pqxdh.mlkem_decapsulate sk ct with
+    | .ok ss => return some ss
+    | _ => return none
+
+def AgreeComm (P : Parameters SPK SSK S C Msg IdC IdK) : Prop :=
+  ∀ kp₁ ∈ support P.ecKeygen, ∀ kp₂ ∈ support P.ecKeygen,
+    pqxdh.x25519_agree kp₁.private_key kp₂.public_key
+      = pqxdh.x25519_agree kp₂.private_key kp₁.public_key
+
+def AgreeTotal (P : Parameters SPK SSK S C Msg IdC IdK) : Prop :=
+  ∀ kp₁ ∈ support P.ecKeygen, ∀ kp₂ ∈ support P.ecKeygen,
+    ∃ z, pqxdh.x25519_agree kp₁.private_key kp₂.public_key = .ok z
+
+def EncapsTotal (P : Parameters SPK SSK S C Msg IdC IdK) : Prop :=
+  ∀ kp ∈ support P.pqKeygen, ∀ coins ∈ support P.encapsCoins,
+    ∃ r, pqxdh.mlkem_encapsulate kp.1 coins = .ok r
+
+def kdfPRF : PRFScheme SS (ECKey × ECKey × ECKey × Option ECKey) (Key × Key × Key) where
+  keygen := $ᵗ SS
+  eval := fun ss q => getOk (deriveKeys q.1 q.2.1 q.2.2.1 q.2.2.2 ss)
+
+def kdfPRFDH (P : Parameters SPK SSK S C Msg IdC IdK) :
+    PRFScheme pqxdh.KeyPair (ECKey × ECKey × Option ECKey × SS) (Key × Key × Key) where
+  keygen := P.ecKeygen
+  eval := fun kp q => getOk (deriveKeys q.1 q.2.1 kp.public_key q.2.2.1 q.2.2.2)
+
+def x25519DH (kp : pqxdh.KeyPair) (pk : ECKey) : ECKey :=
+  getOk (pqxdh.x25519_agree kp.private_key pk)
+
+def genOPK (keygen : ProbComp pqxdh.KeyPair) (hasOPK : Bool) :
+    ProbComp (Option pqxdh.KeyPair) :=
+  if hasOPK then some <$> keygen else pure none
+
+def setup (P : Parameters SPK SSK S C Msg IdC IdK) (msg : Msg) :
+    ProbComp (InitiatorParameters SPK Msg × RecipientIdentity SPK SSK S) := do
+  let ikA ← P.ecKeygen
+  let ikB ← P.ecKeygen
+  let sigkB ← P.sig.keygen
+  let spkB ← P.ecKeygen
+  let spkSigB ← P.sig.sign sigkB.1 sigkB.2 (EncodeEC spkB.public_key)
+  return ({ ikA := ikA, ikB := ikB.public_key, sigpkB := sigkB.1, msg := msg },
+    { ikB := ikB, sigkB := sigkB, spkB := spkB, spkSigB := spkSigB })
+
+def publish (P : Parameters SPK SSK S C Msg IdC IdK)
+    (p : RecipientParameters SPK SSK S) :
+    ProbComp (PreKeyBundle ECKey PQPK S IdC IdK) := do
+  let pqpkSigB ← P.sig.sign p.sigkB.1 p.sigkB.2 (EncodeKEM p.pqpkB.1)
+  return { ikB := p.ikB.public_key
+           spkB := (p.spkB.public_key, P.idEC p.spkB.public_key)
+           spkSigB := p.spkSigB
+           pqpkB := (p.pqpkB.1, P.idKEM p.pqpkB.1)
+           pqpkSigB := pqpkSigB
+           opkB := p.opkB.map fun opk => (opk.public_key, P.idEC opk.public_key) }
+
+def initiate (P : Parameters SPK SSK S C Msg IdC IdK)
+    (p : InitiatorParameters SPK Msg)
+    (bundle : PreKeyBundle ECKey PQPK S IdC IdK) :
+    ProbComp (Option (InitialMessage ECKey CT C IdC IdK ×
+      SessionContext ECKey PQPK Msg Key)) := do
+  if bundle.ikB ≠ p.ikB then return none
+  let okSPK ← P.sig.verify p.sigpkB (EncodeEC bundle.spkB.1) bundle.spkSigB
+  let okPQPK ← P.sig.verify p.sigpkB (EncodeKEM bundle.pqpkB.1) bundle.pqpkSigB
+  if !(okSPK && okPQPK) then return none
+  let ekA ← P.ecKeygen
+  let coins ← P.encapsCoins
+  match pqxdh.pqxdh_initiate
+      { our_identity_key_pair := p.ikA
+        our_ephemeral_key_pair := ekA
+        their_identity_key := bundle.ikB
+        their_signed_pre_key := bundle.spkB.1
+        their_one_time_pre_key := bundle.opkB.map Prod.fst
+        their_kyber_pre_key := bundle.pqpkB.1 } coins with
+  | .ok agreement =>
+      let SK := agreement.keys.root_key
+      let KA := agreement.keys.chain_key
+      let KB := agreement.keys.pqr_key
+      let AD := (p.ikA.public_key, bundle.ikB, bundle.pqpkB.1)
+      let ctxt ← P.aead.encrypt KA AD p.msg
+      return some ({ ikA := p.ikA.public_key
+                     ekA := ekA.public_key
+                     ct := agreement.kyber_ciphertext
+                     idSPK := bundle.spkB.2
+                     idPQPK := bundle.pqpkB.2
+                     idOPK := bundle.opkB.map Prod.snd
+                     ctxt := ctxt },
+        { sk := SK, kb := KB, ad := AD, msg := p.msg })
+  | _ => return none
+
+def accept [DecidableEq IdC] [DecidableEq IdK]
+    (P : Parameters SPK SSK S C Msg IdC IdK)
+    (p : RecipientParameters SPK SSK S)
+    (msg : InitialMessage ECKey CT C IdC IdK) :
+    ProbComp (Option (SessionContext ECKey PQPK Msg Key)) := do
+  if msg.idSPK ≠ P.idEC p.spkB.public_key ∨ msg.idPQPK ≠ P.idKEM p.pqpkB.1 ∨
+      msg.idOPK ≠ p.opkB.map (fun opk => P.idEC opk.public_key) then return none
+  match pqxdh.pqxdh_accept
+      { our_identity_key_pair := p.ikB
+        our_signed_pre_key_pair := p.spkB
+        our_one_time_pre_key_pair := p.opkB
+        our_kyber_secret_key := p.pqpkB.2
+        their_identity_key := msg.ikA
+        their_ephemeral_key := msg.ekA
+        their_kyber_ciphertext := msg.ct } with
+  | .ok (some keys) =>
+      let AD := (msg.ikA, p.ikB.public_key, p.pqpkB.1)
+      match P.aead.decrypt keys.chain_key AD msg.ctxt with
+      | some m =>
+          return some { sk := keys.root_key, kb := keys.pqr_key, ad := AD, msg := m }
+      | none => return none
+  | _ => return none
+
+def confirm [DecidableEq Msg] (P : Parameters SPK SSK S C Msg IdC IdK)
+    (ctx : SessionContext ECKey PQPK Msg Key) (conf : C) : Option Key :=
+  if P.aead.decrypt ctx.kb ctx.ad conf = some ctx.msg then some ctx.sk
+  else none
+
+def initiator [DecidableEq Msg] (P : Parameters SPK SSK S C Msg IdC IdK) :
+    Party ProbComp (InitiatorParameters SPK Msg)
+      (Message ECKey PQPK CT S C IdC IdK) (Option Key) where
+  State := InitiatorParameters SPK Msg ⊕ SessionContext ECKey PQPK Msg Key ⊕ Key
+  init := fun p => pure (.waitForMsg (.inl p))
+  step := fun st w => match st, w with
+    | .inl p, .bundle b => do
+        match ← initiate P p b with
+        | some (im, ctx) => pure (.acceptAndSend (.inr (.inl ctx)) (.initial im) false)
+        | none => pure .reject
+    | .inr (.inl ctx), .confirmation conf =>
+        match confirm P ctx conf with
+        | some SK => pure (.complete (.inr (.inr SK)))
+        | none => pure .reject
+    | _, _ => pure .reject
+  output := fun st => match st with
+    | .inr (.inr SK) => pure (some (some SK))
+    | _ => pure none
+
+def recipient [DecidableEq IdC] [DecidableEq IdK]
+    (P : Parameters SPK SSK S C Msg IdC IdK) (hasOPK : Bool) :
+    Party ProbComp (RecipientIdentity SPK SSK S)
+      (Message ECKey PQPK CT S C IdC IdK) (Option Key) where
+  State := RecipientParameters SPK SSK S ⊕ Key
+  init := fun idn => do
+    let opkB ← genOPK P.ecKeygen hasOPK
+    let pqpkB ← P.pqKeygen
+    let p : RecipientParameters SPK SSK S :=
+      { ikB := idn.ikB, sigkB := idn.sigkB, spkB := idn.spkB, spkSigB := idn.spkSigB,
+        opkB := opkB, pqpkB := pqpkB }
+    let bundle ← publish P p
+    pure (.speakFirst (.inl p) (.bundle bundle))
+  step := fun st w => match st, w with
+    | .inl p, .initial im => do
+        match ← accept P p im with
+        | some ctx => do
+            let conf ← P.aead.encrypt ctx.kb ctx.ad ctx.msg
+            pure (.acceptAndSend (.inr ctx.sk) (.confirmation conf) true)
+        | none => pure .reject
+    | _, _ => pure .reject
+  output := fun st => match st with
+    | .inl _ => pure none
+    | .inr SK => pure (some (some SK))
+
+def uakeInitiator [DecidableEq Msg] [DecidableEq IdC] [DecidableEq IdK]
+    (P : Parameters SPK SSK S C Msg IdC IdK) (msg : Msg) (hasOPK : Bool) :
+    UAKE.Scheme ProbComp Key (InitiatorParameters SPK Msg)
+      (RecipientIdentity SPK SSK S)
+      (Message ECKey PQPK CT S C IdC IdK) where
+  rounds := 3
+  setup := setup P msg
+  U := initiator P
+  T := recipient P hasOPK
+
+def uakeRecipient [DecidableEq Msg] [DecidableEq IdC] [DecidableEq IdK]
+    (P : Parameters SPK SSK S C Msg IdC IdK) (msg : Msg) (hasOPK : Bool) :
+    UAKE.Scheme ProbComp Key (RecipientIdentity SPK SSK S)
+      (InitiatorParameters SPK Msg)
+      (Message ECKey PQPK CT S C IdC IdK) where
+  rounds := 4
+  setup := Prod.swap <$> setup P msg
+  U := recipient P hasOPK
+  T := initiator P
+
+end
+
+end PQXDH.Aeneas.Simplified
