PQXDH/Aeneas2/Extracted/Core.lean
@@ -1,4 +1,0 @@
-import PQXDH.Aeneas2.Extracted.Core.Funs
-import PQXDH.Aeneas2.Extracted.Core.FunsExternal
-import PQXDH.Aeneas2.Extracted.Core.Types
-import PQXDH.Aeneas2.Extracted.Core.TypesExternal
