PQXDH/Aeneas2/Extracted/Protocol.lean
@@ -1,4 +1,0 @@
-import PQXDH.Aeneas2.Extracted.Protocol.Funs
-import PQXDH.Aeneas2.Extracted.Protocol.FunsExternal
-import PQXDH.Aeneas2.Extracted.Protocol.Types
-import PQXDH.Aeneas2.Extracted.Protocol.TypesExternal
