docs/PQXDHDocs/Renderers/MTPMain.lean
@@ -1,5 +1,0 @@
-import PQXDHDocs.Render
-import PQXDHDocs.Chapters.MTP.Overview
-
-def main (args : List String) : IO UInt32 :=
-  PQXDHDocs.renderManual (%doc PQXDHDocs.Chapters.MTP.Overview) args
